\documentclass[a4paper]{article}
\input{preamble.tex}
\usepackage{pdfpages}
\title{Analysis I: Homework 7}
\date{Fri 10 Sep 2021 12:58}
\input{../ops.tex}
\begin{document}
\maketitle
\begin{problem}[31 (Collaborated with Andrea)]
Let \(f = \frac{\sin\left( x \right) }{x}\). We aim to show \(\int f^{+} = \infty\). First, note that \(\int f^{+}  \ge \int_{\left[ 0, \infty \right] } f^{+}\) so it suffices to show this quantity infinite. Moreover, in this interval we find \(f\) positive for \(x \in \left[ 2n\pi, (2n+1)\pi \right] \) for \(n \in \Z^{+}_0\). Hence, defining \(f_{n} = f^{+} \chi_{\left[ 0, \left( 2n+1 \right) \pi \right] }\) we see each \(f_{n}\) is measurable (it is continuous) and non-negative with \(\lim_{n \to \infty}f_{n} \left( x \right) = f^{+}\left( x \right) \) for all \(x \ge 0  \). Moreover, since \(\left[ 0, \left( 2n+1 \right) \pi \right] \subseteq \left[ 0, \left( 2\left( n+1 \right) +1 \right) \pi \right] \) we see \(f_{n} \le f_{n+1}\) for all \(x \in \left[ 0, \infty \right) \).  Hence, applying dominated convergence yields
\begin{align*}
	\int f^{+} &\ge \int _{\left[ 0, \infty \right)} f^{+}\\
	&= \int_{\left[ 0, \infty \right] } \lim_{n \to \infty} f_{n} \\
	&= \lim_{n \to \infty} \int_{\left[ 0, \infty \right] } f_{n} \\
	&= \lim_{n \to \infty} \sum_{i=0}^{n} \int_{\left[ 2i\pi, \left( 2i + 1 \right) \pi \right] } f_{n} \\
	&\ge \lim_{n \to \infty} \sum_{i=0}^{n} \int_{\left[ 2i\pi, \left( 2i+1 \right) \pi \right] } \frac{(\sin ^{+}\left( x \right) \mid_{\left[ 0, 2n\pi \right] })^{*} }{\left( 2i + 1 \right) \pi}\\
	&= \lim_{n \to \infty} \sum_{i=0}^{n} \frac{1}{\left( 2i + 1 \right) \pi } \int_{\left[ 2i\pi, \left( 2i+1 \right) \pi \right] } (\sin^{+}\left( x \right) \mid_{\left[ 0, 2n\pi \right] })^{*}\\
	&\ge \lim_{n \to \infty} \sum_{i=0}^{n} \frac{1}{\left( 2i+1 \right) \pi} \text{ since } \int_{\left[ 2i\pi, \left( 2i+1 \right) \pi \right] } \sin ^{+}\left( x \right) = \int_{\left[ 0, \pi \right] } \sin\left( x \right) = 2 .\\
	&= \frac{1}{\pi} \lim_{n \to \infty} \sum_{i=0}^{n} \frac{1}{\left( 2i+1 \right) }\\
	&= \frac{1}{\pi} \sum_{i= 0}^{\infty} \frac{1}{2i+1} \\
	&=  \infty
.\end{align*}
Hence, \(\int f^{+}\) is not finite, so \(f\) is nonintegrable.
\end{problem}
\newpage
\begin{problem}[32]
	First, note that \(f \coloneqq \frac{1}{\sqrt{x} }\) is measurable (preimage of an interval is an interval) and finite almost everywhere. Then, we define \(A_{n} = \left[ \frac{1}{\left( n-1 \right) ^2}, \frac{1}{n^2} \right] \) and the simple functions \(s_{n} = \sum_{i= 1}^{n} i \chi_{A_{i}}\). As each term is positive, we see \(s_{n}\) is increasing for fixed \(x\). Moreover, \(s = \lim_{n \to \infty}s_{n}\) is integrable by applying DCT
	\begin{align*}
		\int s &= \lim_{n \to \infty} \int s_{n} \\
		&= \lim_{n \to \infty} \sum_{i= 1}^{\infty} \left( \frac{1}{\left( i-1 \right) ^2} - \frac{1}{i^2} \right) i\\
		&= \lim_{n \to \infty} \sum_{i= 1}^{n} \frac{1}{\left( i-1 \right) ^2} + \frac{1}{i\left( i-1 \right) } \\
		&\le \lim_{n \to \infty}\sum_{i= 1}^{n} \frac{2}{i^2}\\
		&= \frac{\pi^2}{3}
	.\end{align*}
	Then, for any \(t \in \mathscr{S}\left( f \right) \) , we see \(t \le s_{n} \le s\) for some \(n = \left\lceil \frac{1}{\sqrt{\inf \{ x : x \in \support\left( t \right)  \} } } \right\rceil \). Hence, \(\int s\) is an upper bound of \(\sup \{ \int t: t \in \mathscr{S}\left( f \right)  \} = \int f \), so \(\int f\) is bounded and hence \(f\) is integrable.
\end{problem}
\newpage
\begin{problem}[33]
	First, basic limits show \(\lim_{n \to \infty}h_{n}\left( x \right)  = \left \{
		\begin{array}{11}
			3, & \quad x \in \left( -1, 1 \right)  \\
			2, & \quad x = -1 \text{ or } x=1\\
			1, & \quad x \in \left( -\infty, -1 \right)\cup \left( 1, \infty \right)
		\end{array}
		\right.\)
		Moreover, \(h_{n}\left( x \right) \) is continuous for every \(n \in \N\), hence measurable. So, we see \\\(h_{n} \cdot f\) is measurable for every \(n \in \N\). Then, \(\lim_{n \to \infty}\left( h_{n} \cdot f \right) \left( x \right) = \left \{
			\begin{array}{11}
				3f\left( x \right) , & \quad x \in \left( -1, 1 \right)  \\
				2f\left( x \right) , & \quad x= \pm 1\\
				f\left( x \right) , &\quad x\in\left( -\infty, -1 \right)\cup \left( 1, \infty \right)
			\end{array}
		\right\). Hence, we see \(\left| h_{n} \cdot f \right|\le 3\left| f \right|  \) with \(3 \left| f \right| \) being integrable (since \(f\) is integrable). Applying dominated convergence yields \[
			\lim_{n \to \infty}\int h_{n} \cdot f = \int \lim_{n \to \infty} h_{n} \cdot f = \int_{\left[ -\infty, -1 \right] } f + \int_{\left[ -1, 1 \right] } 3f + \int_{\left[ 1, \infty \right] } f = \int f \DX  + 2\int_{ \left[ -1, 1 \right] }f \DX
			.\]
\end{problem}
\newpage
\begin{problem}[34]
	First, basic limits again show \(\lim_{n \to \infty}e^{-\frac{x}{n}} = 1\). Moreover, fixing \(x\), we see \(e^{-\frac{x}{n}} < e^{-\frac{x}{n+1}}\), so we see \(e^{-\frac{x}{n}}\left| f \right| \le e^{-\frac{x}{n+1}}\left| f \right| \). Then, denoting \(e^{-\frac{x}{n}}\left| f \right| = f_{n}\), we see \(\lim_{n \to \infty}f_{n} = \lim_{n \to \infty}e^{-\frac{x}{n}} \lim_{n \to \infty}\left| f \right| = \lim_{n \to \infty}\left| f \right| \) with each \(f_{n}\) being measurable (as it is the product of continous functions) and increasing, hence passing to the \(0\)-extension and applying monotone convergence yields \[
	1 \ge \lim_{n \to \infty}\int_{\left( 0, \infty \right) } f_{n} = \lim_{n \to \infty} \int f_{n}^{*} =  \int_{ } \lim_{n \to \infty}f_{n}^{*} = \int_{} (\left| f \right|)^{*} = \int_{\left( 0, \infty \right) } \left| f \right|
	.\]
	Since \(f\) is continuous, we see it is measurable, and since it is absolutely integrable on \(\left( 0, \infty \right) \), we have \(f\) being integrable on \(\left( 0, \infty \right) \).
\end{problem}
\newpage
\begin{problem}[35]
	First, recall \(\sum_{i= 1}^{\infty} \frac{1}{n^{4} } = \frac{\pi^{4}}{90}\).\\
	Then, define \(g_{n} = \sum_{i= 1}^{n} f_{i}^2\) and note that \(g_{n} \le g_{n+1}\) as each term is finite. Moreover \(g_{n}\) is the sum of measurable functions, so it is measurable. Lastly, define \(\lim_{n \to \infty}g_{n}\left( x \right) = g\left( x \right)  = \sum_{i= 1}^{\infty} f_{n}^2\left( x \right) \) Then, monotone convergence  and zero extensions yield
	\begin{align*}
		\int_{\left[ 0, 1 \right] } g = \lim_{n \to \infty} \int_{\left[ 0, 1 \right] }g_{n}
		&= \lim_{n \to \infty}\int g^{*} \\
		&= \lim_{n \to \infty} \int (\sum_{i= 1}^{n} f_{n}^2)^{*} \\
		&= \lim_{n \to \infty} \int_{\left[ 0, 1 \right] } \sum_{i= 1}^{n} f_{n}^2 \\
		&= \lim_{n \to \infty} \sum_{i= 1}^{n} \int_{\left[ 0, 1 \right] }f_{n}^2 \\
		&\le \lim_{n \to \infty} \sum_{i= 1}^{n} \frac{1}{n^{4}} \\
		&= \frac{\pi^{4}}{90} \\
	.\end{align*}
	Moreover, \(0 \le \int_{\left[ 0, 1 \right] }f_{n}^2\) as the integrand is always non-negative. Hence, as the sum is bounded and strictly increasing, we see the terms tend to \(0\). That is \( \lim_{n \to \infty} \int _{\left[ 0, 1 \right] }f_{n}^2 = 0\).
\end{problem}
\end{document}
