\documentclass[a4paper]{article}
\input{../../preamble.tex}
\usepackage{pdfpages}
\title{Algebraic Theory I: Homework III}
\date{Thu 14 Oct 2021 11:07}
\input{../ops.tex}
\begin{document}
\maketitle
\begin{solution}[1]
\begin{enumerate}
	\item First, we note that if \(xK = yK\) for some \(x \neq y\)  , then \(\overline{\phi}\left( xK \right) = \overline{x}H\) and \(\overline{\phi}\left( yK \right) = \overline{y}H\), hence we need to show \(\overline{x}H = \overline{y}H\). We see \(x^{-1}y K = K\), hence \(\overline{\phi}\left( x^{-1}yK \right) = \overline{x^{-1}y}H = \overline{x}^{-1} \overline{y} H = \overline{\phi}\left( 1K \right) = 1 H\). So, \(\overline{x}^{-1}\overline{y} \in H\), hence \(\overline{y} \in \overline{x}H\) and similairly, \(\overline{x} \in\overline{y}H\). So, \(\overline{x}H = \overline{\phi}\left( xK \right) = \overline{y}H = \overline{\phi}\left( yK \right) \), so \(\overline{\phi}\)  is well defined.\\
		Now,
		\begin{align*}
			\overline{\phi}\left( xK yK \right) &= \overline{\phi}\left( xyKK \right)  \\
			&=  \overline{xy} H\\
			&= \phi\left( xy \right) H\\
			&= \phi\left( x \right) \phi\left( y \right) H \\
			&= \overline{x} \overline{y} H\\
			&= \overline{x}\overline{y} H H \text{ as \(H = H H\) by closure }\\
		&= \overline{x} H \overline{y} H \\
		&= \overline{\phi}\left( xK \right) \overline{\phi}\left( yK \right)
		.\end{align*}
		Furthermore, we see \(\overline{\phi}\left( 1K \right) = \overline{1}H = 1H\) as \(\phi\left( 1 \right)  = \overline{1} = 1\)  by homomorphism properties.

			\item  First, note that \(Z_0 \left( \overline{G} \right) = \{1\} = \overline{Z_0\left( G \right) }\). Now, we induce on \(n\) and we see \(Z_{n-1}\left( G \right) \trianglelefteq G\)  and \(Z_{n-1}\left( \overline{G} \right) \trianglelefteq \overline{G}\) with \(\overline{Z_{n-1}\left( G \right) } \le Z_{n-1}\left( \overline{G} \right) \) by inductive hypothesis,  so \(\overline{\phi}: Z_{n}\left( G \right) / Z_{n-1}\left( G \right)  \to Z_{n}\left( \overline{G} \right) / Z_{n-1}\left( \overline{G} \right) \) is a well defined homomorphism. Hence, letting \(\overline{x} \in \overline{Z_{n}\left( G \right) }\), hence \(x \in Z_{n}\left( G \right) \) and hence \(xZ_{n-1}\left( G \right)  \in Z_{n}\left( G \right) / Z_{n-1}\left( G \right) \)  implies \(\overline{\phi}xZ_{n-1}\left( G \right)  = \overline{x}Z_{n-1}\left( \overline{G} \right) \in Z_{n}\left( \overline{G} \right) / Z_{n-1}\left( \overline{G} \right)  \) . Hence, we find \(\overline{x} \in Z_{n}\left( \overline{G} \right) \). This completes the induction.
			\item Suppose \(G\) is nilpotent and let \(n\) be the nilpotence class of \(G\). Then, we see \(\overline{Z_{n}\left( G \right) } = \overline{G} \le Z_{n}\left( \overline{G} \right) \). Hence, \(\overline{G}\) is of nilpotence class at most \(n\), so we see \(\overline{G}\) is nilpotent.
			\item Let \(\overline{G} = H\) with \(\phi: G \to H\)  being the restriction to \(H\) homomoprhism. That being \(\phi\left( x \right)  = \left \{
				\begin{array}{11}
					x, & \quad x \in H \\
					1, & \quad x \not\in H
				\end{array}
				\right.\) It is clear this is well defined
				\item Suppose \(n\) is the nilpotence class of \(G\). Then \(Z_{n}\left( G \right) \cap H = G \cap H = H \le Z_{n}\left( H \right) \), so \(H\) is of nilpotence class at most \(n\), hence \(H\) is nilptent.
\end{enumerate}
\end{solution}
\newpage
\begin{lemma}
	Automorphisms preserve maximality of subgroups.\\
	Let \(\phi :G \to G\)  be an automorphism and let \(M < G\)  be a maximal subgroup. Suppose \(\phi\left( M \right) = M^{\prime} \) is not maximal. That is, there is a \(\overline{M}^{\prime}\)  such that \(M^{\prime} < \overline{M}^{\prime} < G\). Then, we find
	\begin{align*}
		\phi ^{-1}\left( \overline{M}^{\prime} \right) &=  \phi ^{-1} \left( M^{\prime} \cup \left( \overline{M}^{\prime} \setminus M^{\prime} \right)\right)  \\
							       &= \phi ^{-1}\left( M^{\prime} \right) \cup \phi ^{-1}\left( \overline{M}^{\prime} \setminus M^{\prime}\right)  \\
							       &= M \cup \{\phi^{-1}\left( m \right) : m \in \overline{M}^{\prime} \setminus M^{\prime}\}  \\
							       &> M
	.\end{align*}
Furthermore, \(\overline{M}^{\prime} < G\)  by assumption, hence \(M < \overline{M}^{\prime} < G\). \(\lightning\) .
\end{lemma}
\begin{solution}[2]
	\begin{proof}
		Now, let \(\alpha: G \to G\)  be an automorphism of \(G\) and denote \(\alpha \left( M \right)  = M^{\prime}\) . Then, we see
\begin{align*}
\alpha \left( \Phi \left( G \right)  \right)  &= \alpha\left( \bigcap_{\underset{M \text{ is maximal}}{M < G}} M \right)  \\
						      &= \bigcap_{ \underset{ M \text{ is maximal}}{M < G}} \alpha \left( M \right)   \\
						      &= \bigcap_{\underset{M \text{ is maximal}}{M < G}} M^{\prime} \\
.\end{align*}
Then, as \(M^{\prime}\) is maximal and \(\alpha\) is an injection, we see if \(N \neq M\) are both maximal subgroups, we have \(\alpha \left( N \right)  \neq \alpha \left( M \right) \), hence \[\{ M :  \underset{ M \text{ is maximal}}{M < G}\}  = \{M^{\prime} :  \underset{ M \text{ is maximal}}{M < G}\} .\] So, we have \[
	\alpha\left( \Phi \left( G \right)  \right)  = \bigcap_{ \underset{ M \text{ is maximal}}{M < G}} M^{\prime} = \bigcap_{ \underset{ M \text{ is maximal}}{M < G}} M = \Phi\left( G \right)
.\]
\end{proof}
\end{solution}
\newpage
\begin{solution}[3]

\end{solution}
\newpage
\begin{solution}[4]
	\begin{lemma}
		\(\left[ M, M \right] \)  and \(\left<x^{p} : x \in M \right> \)  are characteristic in \(M\).\\
		Let \(\alpha: M \to M\) be an automorphism. Then, denote \(\alpha\left( x \right)  = x^{\prime}\)  for \(x \in M\) and we see,
		\begin{align*}
			\alpha\left( \left[ M, M \right]  \right) &= \alpha\left( \left<xyx^{-1}y^{-1} : x, y \in M \right> \right)  \\
								  &= \left<\alpha\left( xyx^{-1}y^{-1} \right) x, y \in M \right>  \\
								  &= \left<\alpha\left( x \right) \alpha\left( y \right) \alpha\left( x \right) ^{-1} \alpha\left( y \right)^{-1} : x, y \in M  \right>  \\
								  &= \left<x^{\prime} y^{\prime} x^{\prime}^{-1} y^{\prime}^{-1} : x, y \in M \right>  \\
								  &\le \left<x^{\prime}y^{\prime}x^{\prime}^{-1}y^{\prime}^{-1} : x^{\prime}, y^{\prime} \in  M \right>  \\
								  &=  \left[ M, M \right]
		.\end{align*}
		Similairly,
		\begin{align*}
			\alpha \left( \left<x^{p} : x\in M \right>  \right) &= \left<\alpha\left( x^{p} \right): x \in M  \right>  \\
									    &= \left<\alpha\left( x \right) ^{p} : x \in M \right>  \\
									    &= \left<x^{\prime}^{p} : x \in M \right>  \\
									    &\le \left<x^{\prime}^{p} : x^{\prime} \in M \right>
									    &= \left<x^{p} : x \in M \right>  \\
		.\end{align*}
Then, we see as \(M \trianglelefteq G\) and these two groups are characteristic we also have \(\left<x^{p}: x\in M \right> \trianglelefteq G \) and \(\left[ M, M \right] \trianglelefteq G\). Furthermore, we note that as \(xyx^{-1}y^{-1} \in M\)  for \(x, y \in M\) we have \(\left\{ M, M \right\}  \le \left<x^{p}: x\in M \right> \). Now,
Suppose \(M\) is not an elementary abelian \(p\)-group. Then, we find either \(\left[ M, M \right] > 1\)  or there is an element \(x\) of order \(q \neq p\).
	\end{lemma}
\end{solution}
\newpage
\begin{solution}[5]


\end{solution}
\end{document}
